theories/Environment.v
@@ -1,0 +1,51 @@
+Require Import Blech.Spec.
+Require Import Blech.SpecNotations.
+
+Require Import Coq.Unicode.Utf8.
+Require Coq.Lists.List.
+
+Require Import FunInd.
+
+Import List.ListNotations.
+Import IfNotations.
+
+Implicit Type Γ: environment.
+Implicit Type t: type.
+Implicit Types x y: var.
+
+Function find x Γ :=
+  if Γ is ((y, t) :: T)%list
+  then
+    if eq_var x y
+    then
+      Some t
+    else
+      find x T
+  else
+    None.
+
+Lemma find_sound:
+  ∀ {x Γ t}, find x Γ = Some t → mem x t Γ.
+Proof using .
+  intros x Γ.
+  functional induction (find x Γ).
+  all: intros ? p.
+  all: inversion p.
+  all: subst.
+  all: constructor.
+  all: auto.
+Qed.
+
+Lemma find_complete {x Γ t}:
+  mem x t Γ → find x Γ = Some t.
+Proof using .
+  intro p.
+  induction p.
+  all: cbn.
+  - destruct eq_var.
+    2: contradiction.
+    reflexivity.
+  - destruct eq_var.
+    1: contradiction.
+    auto.
+Qed.
